examples/PolyRewrite/MSimpleMonads.v
@@ -1,0 +1,158 @@
+(** This is a very simple monadic language that
+ ** can be useful for testing.
+ **)
+Require Import ExtLib.Core.RelDec.
+Require Import ExtLib.Data.Fun.
+Require Import ExtLib.Data.Nat.
+Require Import ExtLib.Tactics.
+Require Import MirrorCore.ExprI.
+Require Import MirrorCore.TypesI.
+Require Import MirrorCore.SymI.
+Require Import MirrorCore.MTypes.ModularTypes.
+Require Import MirrorCore.MTypes.TSymOneOf.
+
+Set Implicit Arguments.
+Set Strict Implicit.
+
+Inductive typ' : nat -> Type :=
+| tyNat : typ' 0
+| tyBool : typ' 0
+| tyMonad : typ' 1.
+
+Definition typ'_dec n (a : typ' n) : forall b : typ' n, {a = b} + {a <> b}.
+refine
+  match a as a in typ' n return forall b : typ' n, {a = b} + {a <> b} with
+  | tyNat => fun b =>
+              match b as b in typ' k return (match k return typ' k -> Type with
+                                             | 0 => fun t => {tyNat = t} + {tyNat <> t}
+                                             | _ => fun _ => unit end b) with
+               | tyNat => left eq_refl
+               | tyBool => right _
+               | tyMonad => tt
+               end
+  | tyBool => fun b =>
+               match b as b in typ' 0 return {_ = b} + {_ <> b} with
+               | tyBool => left eq_refl
+               | tyNat => right _
+               end
+  | tyMonad => fun b =>
+               match b as b in typ' 1 return {tyMonad = b} + {tyMonad <> b} with
+               | tyMonad => left eq_refl
+               end
+  end; try (intro H; inversion H).
+Defined.
+
+Require Import ExtLib.Structures.Monad.
+Section Monad.
+    Variable M : Type -> Type.
+    Variable M_mon : Monad M.
+
+    Instance TSym_typ' : TSym typ' :=
+      { symbolD n s :=
+          match s with
+          | tyNat => nat
+          | tyBool => bool
+          | tyMonad => M
+          end
+        ; symbol_dec := typ'_dec }.
+
+    Definition typ := mtyp typ'.
+
+    Global Instance RType_typ : RType typ := RType_mtyp _ _.
+    Global Instance RTypeOk_typ : @RTypeOk _ RType_typ := RTypeOk_mtyp _ _.
+
+    Inductive func :=
+    | Lt | Plus | N : nat -> func | Eq : typ -> func
+    | Ex : typ -> func | All : typ -> func
+    | And | Or | Impl | Bind : typ -> typ -> func | Ret : typ -> func.
+
+    Local Notation "! x" := (@tyBase0 _ x) (at level 0).
+
+    Print mtyp.
+
+    Definition typeof_func (f : func) : option typ :=
+      Some match f with
+           | Lt => tyArr !tyNat (tyArr !tyNat !tyBool)
+           | Plus => tyArr !tyNat (tyArr !tyNat !tyNat)
+           | N _ => !tyNat
+           | Eq t => tyArr t (tyArr t tyProp)
+           | And | Or | Impl => tyArr tyProp (tyArr tyProp tyProp)
+           | Ex t | All t => tyArr (tyArr t tyProp) tyProp
+           | Bind alpha beta => tyArr (tyBase1 tyMonad alpha) (tyArr (tyArr alpha (tyBase1 tyMonad beta)) (tyBase1 tyMonad beta))
+           | Ret alpha => tyArr alpha (tyBase1 tyMonad alpha)
+           end.
+
+    Definition funcD (f : func)
+      : match typeof_func f with
+        | None => unit
+        | Some t => typD t
+        end :=
+      match f as f return match typeof_func f with
+                          | None => unit
+                          | Some t => typD t
+                          end
+      with
+      | Lt => NPeano.Nat.ltb
+      | Plus => plus
+      | N n => n
+      | Eq t => @eq _
+      | And => and
+      | Or => or
+      | Impl => fun (P Q : Prop) => P -> Q
+      | All t => fun P => forall x : typD t, P x
+      | Ex t => fun P => exists x : typD t, P x
+      | Bind a b => bind
+      | Ret a => ret
+      end.
+
+    Let RelDec_eq_typ : RelDec (@eq typ) := RelDec_Rty _.
+    Local Existing Instance RelDec_eq_typ.
+
+    Instance RelDec_eq_func : RelDec (@eq func) :=
+      { rel_dec := fun (a b : func) =>
+                     match a , b with
+                     | Plus , Plus => true
+                     | Lt , Lt => true
+                     | N a , N b => a ?[ eq ] b
+                     | Eq a , Eq b => a ?[ eq ] b
+                     | And , And
+                     | Impl , Impl
+                     | Or , Or => true
+                     | All a , All b
+                     | Ex a , Ex b => a ?[ eq ] b
+                     | Bind a b, Bind a' b' => andb (a ?[eq] a') (b ?[eq] b')
+                     | Ret a, Ret a' => a ?[eq] a'
+                     | _ , _ => false
+                     end
+      }.
+
+
+    Instance RelDecCorrect_eq_func : RelDec_Correct RelDec_eq_func.
+    Proof.
+      constructor.
+      destruct x; destruct y; simpl;
+      try solve [ tauto
+                | split; congruence
+                | rewrite rel_dec_correct; split; congruence
+                ].
+      split.
+      { intros. apply andb_prop in H. destruct H.
+        rewrite rel_dec_correct in H. rewrite rel_dec_correct in H0.
+        subst; auto. }
+      { intros. inversion H. subst.
+        do 2 (rewrite rel_dec_eq_true; [|eauto with typeclass_instances|reflexivity]).
+        reflexivity. }
+    Qed.
+
+    Instance RSym_func : RSym func :=
+      { typeof_sym := typeof_func
+        ; symD := funcD
+        ; sym_eqb := fun a b => Some (a ?[ eq ] b)
+      }.
+
+    Instance RSymOk_func : RSymOk RSym_func.
+    { constructor.
+      intros. simpl. consider (a ?[ eq ] b); auto. }
+    Qed.
+
+End Monad.
